ghost state...

snglswch/lucid_base_rec.dfy
@@ -7,16 +7,24 @@ abstract module LucidBase {
     const T : nat := 256
     type Event (==)
     datatype LocEvent = LocEvent(e : Event, time : bits, natTime : nat)
+
+    class GState {
+        ghost constructor ()
+            ensures fresh(this)
+        { }
+    }
+
     class State {
         constructor () 
             ensures fresh(this)
         { }
     }
-    class Handlers { // maybe should be "prog" or something. Not just handlers, really.
+    class Handlers {
 
 
         // state and event queue are mutable for user-facing abstractions
         var state : State
+        ghost var gState : GState
         var queue : seq<LocEvent> // event * timestamp
 
         var time    : bits // We need time as a class variable because we want an 
@@ -28,19 +36,20 @@ abstract module LucidBase {
 
         /***   user-defined predicates   ***/
         // an invariant over the last event that was processed, the current event, and the remaining events
-        ghost predicate inter_event_invariant(s : State, cur_ev : LocEvent, ev_queue : seq<LocEvent>, lastNatTime : nat)
-            reads s
+        ghost predicate inter_event_invariant(s : State, gs : GState, cur_ev : LocEvent, ev_queue : seq<LocEvent>, lastNatTime : nat)
+            reads s, gs
 
         // post_dispatch must hold at the end of every event handler's execution
-        ghost predicate post_dispatch(s : State, updated_queue : seq<LocEvent>, processed_event_natTime : nat)
-            reads s
+        ghost predicate post_dispatch(s : State, gs : GState, updated_queue : seq<LocEvent>, processed_event_natTime : nat)
+            reads s, gs
         {
                 |updated_queue| > 0 ==> 
-                        inter_event_invariant(s, updated_queue[0], updated_queue[1..], processed_event_natTime)            
+                        inter_event_invariant(s, gs, updated_queue[0], updated_queue[1..], processed_event_natTime)            
         }
         // a predicate that must hold over the entire event queue before and after 
         // dispatch, that defines the pairs of events that we may see
         ghost predicate valid_next_event(cur : LocEvent, next : LocEvent)
+        
 
         ghost predicate valid_event_queue(ev_queue : seq<LocEvent>)
         {
@@ -77,20 +86,20 @@ abstract module LucidBase {
 
         lemma valid_event_queue_implies_valid_time(ev_queue : seq<LocEvent>)
             requires valid_event_queue(ev_queue)
-            requires |ev_queue| > 0
-            ensures  ev_queue[0].time == ev_queue[0].natTime % T
+            ensures  |ev_queue| > 0 ==> ev_queue[0].time == ev_queue[0].natTime % T
 
         constructor ()
 
         method ProcessEvent(i : nat, eq : seq<LocEvent>) returns (j : nat)
             requires |eq| > 0
             requires valid_event_queue(eq)
-            requires inter_event_invariant(this.state, eq[0], eq[1..], lastNatTime)
+            requires inter_event_invariant(this.state, this.gState, eq[0], eq[1..], lastNatTime)
             requires lastNatTime <= eq[0].natTime
             requires this.natTime == eq[0].natTime
             requires this.time == eq[0].time
-            modifies this`queue, this.state, this`lastNatTime, this`natTime, this`time
+            modifies this`queue, this.state, this`lastNatTime, this`natTime, this`time, this.gState
         {
+            
             valid_event_queue_implies_valid_time(eq);
             assert (eq[0].time == eq[0].natTime % T);
             if (i <= 0) {
@@ -100,7 +109,7 @@ abstract module LucidBase {
                 var ev_head := eq[0];
                 var eq_tail := eq[1..];
                 this.queue := eq_tail;
-                assert inter_event_invariant(this.state, ev_head, queue, lastNatTime);                
+                assert inter_event_invariant(this.state, this.gState, ev_head, queue, lastNatTime);                
                 Dispatch(ev_head);
                 // if the queue is now empty, we are done
                 if (queue == []) {
@@ -133,14 +142,20 @@ abstract module LucidBase {
             }
         }
 
+        predicate correct_internal_time(cur_ev : LocEvent)
+            reads this`natTime, this`time
+        {
+            this.natTime == cur_ev.natTime
+            && this.time    == cur_ev.time
+            && this.time    == this.natTime % T            
+        }
         method Dispatch(cur_ev : LocEvent)
-            modifies this.state, this`queue
+            modifies this.state, this.gState, this`queue
             // at the start of dispatch, the user event invariant must hold for the current event
-            requires inter_event_invariant(this.state, cur_ev, this.queue, this.lastNatTime)
+            requires inter_event_invariant(this.state, this.gState, cur_ev, this.queue, this.lastNatTime)
             // and the event must be part of a valid sequence of events
             requires valid_event_queue([cur_ev] + this.queue)
-            requires this.natTime == cur_ev.natTime
-            requires this.time    == this.natTime % T
+            requires correct_internal_time(cur_ev)
             requires this.natTime >= this.lastNatTime
             // after processing, if the queue has more items in it to process, 
             // then the user event invariant holds over:
@@ -158,7 +173,7 @@ abstract module LucidBase {
                 maybe we can do something weaker / simpler: 
                 if there's an event in the queue, then it must be a valid next event and the inter-event invariant must hold?
             */
-            ensures post_dispatch(state, queue, natTime)
+            ensures post_dispatch(state, gState, queue, natTime)
             // and the event must still be part of a valid sequence of events
             // is this necessary any more?
             ensures  valid_event_queue([cur_ev] + this.queue)
