snglswch/snglswch5_rec.dfy
@@ -2,33 +2,43 @@ include "lucid_base_rec.dfy"
 
 module LucidProg refines LucidBase {
 
-    datatype Event = 
+   datatype Event = 
       // | NOOP()
       | ProcessPacket(dnsRequest: bool, uniqueSig: nat)
       | SetFiltering(on : bool)
-      
+
       // | SetFiltering(on : bool)
       // | ProcessPacket(dnsRequest: bool, uniqueSig: nat)
       // | PacketOut() // optional.
 
-    class State ... {
+
+   class GState ... {
+      ghost var requestSet : set<nat>   // pending requests, for filtering
+      // ghost variables for reasoning about timeOn
+      ghost var actualTimeOn : nat 
+      ghost var natTimeOn : nat    
+      ghost var preFilterSet : set<nat> // requestSet, before any deletion
+      // ghost var recircSwitch : bool 
+
+      ghost constructor ()
+            ensures actualTimeOn == 0
+            ensures natTimeOn == 0
+            ensures requestSet == {}
+      {
+         actualTimeOn, natTimeOn := 0, 0;
+         requestSet := {};
+      }
+   }
+
+   class State ... {
       // Address State 
       var lastIntv : bits    // an interval, so first 8-i bits always zero
       var count : nat                           // counter for DNS replies
       var filtering : bool          // turns adaptive filtering on and off
       var timeOn : bits      // implementation of time filtering turned on
       var recircPending : bool          // a "semaphore" for recirculation
-      ghost var requestSet : set<nat>   // pending requests, for filtering
 
-      // ghost variables for reasoning about timeOn
-      ghost var actualTimeOn : nat 
-      ghost var natTimeOn : nat
-      const T : nat := 256
 
-      
-
-      ghost var preFilterSet : set<nat> // requestSet, before any deletion
-      // ghost var recircSwitch : bool 
 
       constructor ()
             ensures (this.filtering == false)
@@ -39,14 +49,9 @@ module LucidProg refines LucidBase {
             ensures lastIntv == 0
             ensures count == 0
             ensures timeOn == 0
-            ensures actualTimeOn == 0
-            ensures natTimeOn == 0
-            ensures requestSet == {}
       {
          filtering, recircPending := false, false;
          lastIntv, count, timeOn := 0, 0, 0;
-         actualTimeOn, natTimeOn := 0, 0;
-         requestSet := {};
       }
     }
    // Parameters
@@ -66,12 +71,16 @@ module LucidProg refines LucidBase {
             requires QRoff > Q
             requires W >= Q
             ensures (fresh(state))
+            ensures (fresh(gState))
             // does not establish inter-event invariant
             // because the event queue is empty
       {     
              state := new State();   
+             gState := new GState();
              queue := [];
       } 
+
+
 
       predicate parameterConstraints ()      // from problem domain, ghost  
       {  I > 0 && QRoff > Q > 0  && W >= Q  }
@@ -79,42 +88,59 @@ module LucidProg refines LucidBase {
 
       ghost predicate valid_next_event(cur : LocEvent, next : LocEvent)
       {
-         next.natTime - cur.natTime < T - I
+         (next.natTime - cur.natTime < T - I)
       }
 
 
       /*** the inter-event invariant ***/
-      ghost predicate inter_event_invariant(s : State, cur_ev : LocEvent, ev_queue : seq<LocEvent>, lastNatTime : nat)
+      ghost predicate inter_event_invariant(s : State, gs : GState, cur_ev : LocEvent, ev_queue : seq<LocEvent>, lastNatTime : nat)
       {
          var natTime := cur_ev.natTime;
          parameterConstraints()
          && (natTime - lastNatTime < T - I)
-         // && (natTime < s.actualTimeOn + T) // TODO: I don't understand this predicate.
-         // Seems like there are some input sequences that are valid, 
-         // but for which this would not hold
+         && stateInvariant(s, gs, ev_queue, cur_ev.time, cur_ev.natTime, lastNatTime)
+         // && (natTime < s.actualTimeOn + T)
+         // Left off here. This is really weird requirement. 
+         // the event's timestamp has to be within a rollover of 
+         // actualTimeOn.
+         // What if filtering never gets turned on?
+         // Or, what if filtering turns on and never shuts off? 
+         // In either case, I think there's a "hard" limit on the time that the events may have. 
+         // they have to be within T of when filtering turned on.
+
+         // Its not an inter-arrival limit. 
+         // And it depends on the state. 
+         // LEFT OFF HERE:
+         // So lets try to work that in tomorrow. A "valid event" constraint that 
+         // just forces all the events in the queue to have less than the current state's actualTimeOn + T, 
+         // (maybe only if the current state says filtering is on?)
+         // I think that will be okay-ish. 
+         // The discuss doubts with Pamela
       }
-      ghost predicate stateInvariant (state : State, es : seq<Event>, time : bits, natTime : nat, lastNatTime : nat)         // ghost
-         reads state
+      ghost predicate stateInvariant (state : State, gstate : GState, es : seq<LocEvent>, time : bits, natTime : nat, lastNatTime : nat)         // ghost
+         reads state, gstate
       {
          // CHANGE: lastNatTime --> natTime because it doesn't make sense in 
          //         SetFiltering (it sets natTimeOn to the current time, not the last time)
-              (  state.natTimeOn <= natTime  ) 
-         && (  state.timeOn == state.natTimeOn % T  )
-         && (  state.natTimeOn >= state.actualTimeOn  )
+              (  gstate.natTimeOn <= natTime  ) 
+         && (  state.timeOn == gstate.natTimeOn % T  )
+         && (  gstate.natTimeOn >= gstate.actualTimeOn  )
          && (  state.filtering ==> 
-                  (protecting (state, natTime) <==> protectImplmnt (state, time))  )
-         && (  ! state.filtering ==> state.requestSet == {}  )
+                  (protecting (state, gstate, natTime) <==> protectImplmnt (state, time))  )
+         && (  ! state.filtering ==> gstate.requestSet == {}  )
          // && (  state.recircPending ==> (state.filtering == ! state.recircSwitch)  )
          // && recircInvariant(state, es) // TODO: add recircInvariant back in
       }
-      ghost predicate protecting (state : State, natTime : nat)  
-      reads state                        // ghost
-      {  state.filtering && (natTime >= state.natTimeOn + Q as nat)  }
+
+      ghost predicate protecting (state : State, gstate : GState, natTime : nat)  
+      reads state, gstate
+                              // ghost
+      {  state.filtering && (natTime >= gstate.natTimeOn + Q as nat)  }
 
       predicate protectImplmnt (state : State, time: bits)
+      reads state
       // protecting is a specification, using history variables.  This
       // is its implementation, which cannot use history variables.
-      reads state
       {  state.filtering && elapsedTime (time, state.timeOn) >= Q  } 
 
       function elapsedTime (now: bits, origin: bits): (res: bits)
@@ -130,41 +156,35 @@ module LucidProg refines LucidBase {
 
       method Dispatch(cur_ev : LocEvent)
       {
-         assert cur_ev.natTime == this.natTime;
-         assert this.time == (this.natTime % T);
-         
-         if
-            // case cur_ev.e.NOOP? => {}
-            case cur_ev.e.ProcessPacket? => {
-               var fwd := processPacket(cur_ev);
-            }
-            case cur_ev.e.SetFiltering? => { 
-               valid_event_queue_implies_valid_head([cur_ev] + this.queue);
-            }
+
       }
 
+
+
+
       method processPacket (cur_ev : LocEvent) returns (forwarded: bool)  
-         modifies this.state, this`queue
+         modifies this.state, this`queue, this.gState
          requires cur_ev.e.ProcessPacket? 
          requires valid_event_queue([cur_ev] + this.queue)
-         requires inter_event_invariant(state, cur_ev, this.queue, this.lastNatTime)
-         requires cur_ev.natTime == this.natTime
+         requires inter_event_invariant(state, gState, cur_ev, this.queue, this.lastNatTime)
+         requires correct_internal_time(cur_ev)
 
          /* pasting in requirements from old version -- TODO: what's necessary? */
-         requires time == natTime % T
          requires natTime >= lastNatTime
          requires natTime - lastNatTime < T - I
+         
 
-         ensures (  ! cur_ev.e.dnsRequest && protecting (state, natTime)
-               && (! (cur_ev.e.uniqueSig in state.preFilterSet))      )
+         ensures (  ! cur_ev.e.dnsRequest && protecting (state, gState, natTime)
+               && (! (cur_ev.e.uniqueSig in gState.preFilterSet))      )
                ==> ! forwarded   // Adaptive Protection, needs exactness
 
          // ensures ! forwarded ==>                           // Harmlessness
          //       (  ! e.dnsRequest && (! (e.uniqueSig in state.preFilterSet))  )
-         ensures post_dispatch(state, queue, natTime)
+         // ensures post_dispatch(state, queue, natTime)
          // requires natTime < state.actualTimeOn + T // See note in inter-event invariant
-         ensures  valid_event_queue([cur_ev] + this.queue)
+         // ensures  valid_event_queue([cur_ev] + this.queue)
       {
+
          // 
          if (cur_ev.e.dnsRequest) {
             forwarded := false;
@@ -196,32 +216,81 @@ module LucidProg refines LucidBase {
             // so this is defensive programming.)  There is no declarative 
             // specification of turning filtering off,  so we make the code as 
             // readable as possible.
-               var tmpFiltering : bool := state.filtering;                // get memop
-               var tmpTimeOn : bits;
-               var tmpRecircPending : bool;
-               if ! tmpFiltering {
-                  if tmpCount >= U {
-                     // time to turn filtering on
-                     tmpRecircPending := state.recircPending;     // get memop . . . .
-                     state.recircPending := true;                 // with update memop
-                     if ! tmpRecircPending {
-                        // IF LUCID
-                        // generate SetFiltering (true);
-                        // ELSE
-                        // state.recircSwitch := true;                           // ghost
-                        // TODO: refactor so that generate doesn't need these extra arguments
-                        Generate(cur_ev, SetFiltering(true), next_generate_time(natTime, queue));                        
-                     }
+            var tmpFiltering : bool := state.filtering;                // get memop
+            var tmpTimeOn : bits;
+            var tmpRecircPending : bool;
+            if ! tmpFiltering {
+               if tmpCount >= U {
+                  // time to turn filtering on
+                  tmpRecircPending := state.recircPending;     // get memop . . . .
+                  state.recircPending := true;                 // with update memop
+                  if ! tmpRecircPending {
+                     // IF LUCID
+                     // generate SetFiltering (true);
+                     // ELSE
+                     // state.recircSwitch := true;                           // ghost
+                     // TODO: refactor so that generate doesn't need these extra arguments
+                     Generate(cur_ev, SetFiltering(true), next_generate_time(natTime, queue));                        
+                     // FI
+                  }  // else recirc already generated, do nothing
+               }  
+            }
+            else { // filtering
+               if oldCount != 0 { // interval boundary crossed
+                  if oldCount >= L {
+                     if elapsedTime (time, state.timeOn) >= Q        // get memop .
+                        {  tmpTimeOn := (time - Q) % T;  }     // . . . . . .
+                     else { tmpTimeOn := state.timeOn; }             // . . . . . .
+                     if elapsedTime (time, state.timeOn) >= Q {      // with update
+                        
+                     /*
+                        BREAKS HERE -- need state invariant!
+                     */
+                        assert natTime - Q >= 0;
+                        state.timeOn := (time - Q) % T;              // memop 
+                        gState.natTimeOn := natTime - Q;                    // ghost
+                     }                                           
                   }
-               }
-            forwarded := false;
-         }
+                  else { // oldCount < L
+                     tmpTimeOn := state.timeOn;                        // get memop
+                     if elapsedTime (time, tmpTimeOn) >= QRoff {
+                        // time to turn filtering off
+                        tmpRecircPending := state.recircPending;//get memop . . . .
+                        state.recircPending := true;           // with update memop
+                        if ! tmpRecircPending {
+                           // IF LUCID
+                           // generate SetFiltering (false);
+                           // ELSE
+                           // state.recircSwitch := false;                    // ghost
+                           // TODO: refactor so that generate doesn't need these extra arguments
+                           Generate(cur_ev, SetFiltering(false), next_generate_time(natTime, queue));                        
+                           // FI
+                        }  // else recirc already generated, do nothing
+                     }
+                  }  
+               } // end boundary-crossing case
+               else {  tmpTimeOn := state.timeOn; }                    // get memop
+            } // end filtering case
 
-         valid_event_queue_implies_valid_head([cur_ev] + this.queue);
-         assert (
-            |queue| > 0 ==> 
-               (inter_event_invariant(state, queue[0], queue[1..], natTime))
-         );
+            // Filtering decision:
+            // if filtering off, it won't matter that timeOn not read
+            if tmpFiltering && elapsedTime (time, tmpTimeOn) >= Q {
+               forwarded := false;//   filter (dnsRequest, uniqueSig);
+            }
+            else {  forwarded := true; }
+         } // end !dnsRequest (processResponse body)
+
+               // assert (prot_clause == prot_impl_clause);
+
+               // assert (protecting (state, queue[0].natTime) <==> protectImplmnt (state, queue[0].time));
+            // }
+         
+
+         // assert (
+         //    |queue| > 0 ==> 
+         //       (inter_event_invariant(state, queue[0], queue[1..], natTime))
+         // );
+         // assert post_dispatch (state, this.queue, cur_ev.natTime);
          
       }
     }
